Test.dfy
@@ -1,5 +1,8 @@
+include "AVLnode.dfy"
 include "AVLtree.dfy"
 
 method Test() {
     var avlTree: AVLtree := new AVLtree();
+    var avlNode: AVLnode := new AVLnode(3);
+    assert(avlNode.balanced());
 }
